NumLean/Meta/ForAll.lean
@@ -1,4 +1,4 @@
 import NumLean.Meta.ForAll.Basic
-import NumLean.Meta.ForAll.RcoNat
+import NumLean.Meta.ForAll.RcoNative
 import NumLean.Meta.ForAll.HTuple
 import NumLean.Meta.ForAll.Notation
